Common interface

interface/Map_extended.fst
@@ -94,3 +94,11 @@ let lemma_InIterUpd #key #val1 #val2 f m k = ()
 let lemma_InDomRestrict #key #value m ks k = ()
 let lemma_ContainsDom #key #value m k      = ()
 let lemma_UpdDomain #key #value m k v      = ()
+
+let equal (#key:eqtype) (#value:Type) (m1:t key value) (m2:t key value) : Type0 =
+    F.feq m1.mappings m2.mappings /\
+    S.equal m1.domain m2.domain
+
+let lemma_equal_intro #key #value m1 m2 = ()
+let lemma_equal_elim #key #value m1 m2  = ()
+let lemma_equal_refl #key #value m1 m2  = ()
