interface/Set_extended_old.fst
@@ -29,8 +29,7 @@ let union (#a:eqtype) (s1:set a) (s2:set a) =
   List.Tot.Base.append s1 s2
 
 let union_mem (#a:eqtype) (s1:set a) (s2:set a) (x:a)
-  : Lemma (ensures (mem x (union s1 s2) <==> (mem x s1 \/ mem x s2)) /\
-                   (not (mem x (union s1 s2)) <==> (not (mem x s1) /\ not (mem x s2)))) =
+  : Lemma (ensures mem x (union s1 s2) <==> (mem x s1 \/ mem x s2)) =
   append_mem_forall s1 s2
 
 let rec remove (#a:eqtype) (ele:a) (s1:set a) : (r:set a{forall e. mem e r <==> mem e s1 /\ e <> ele}) =
@@ -50,6 +49,26 @@ let rec intersect_mem (#a:eqtype) (s1:set a) (s2:set a) (x:a)
   |[] -> ()
   |x1::xs -> if mem x1 s2 then intersect_mem xs (remove x1 s2) x else intersect_mem xs s2 x
 
+let rec difference (#a:eqtype) (s1:set a) (s2:set a) =
+  match s1 with
+  |[] -> []
+  |x::xs -> if mem x s2 then difference xs s2 else x::difference xs s2
+
+let rec mem_difference (#a:eqtype) (s1 s2:set a) (x:a)
+  : Lemma (ensures mem x (difference s1 s2) <==> (mem x s1 /\ ~ (mem x s2)))
+          (decreases s1) =
+  match s1 with
+  |[] -> ()
+  |x1::xs -> if mem x1 s2 then mem_difference xs s2 x else mem_difference xs s2 x
+
+let mem_subset (#a:eqtype) (s1 s2:set a)
+  : Lemma (requires (forall x. mem x s1 ==> mem x s2))
+          (ensures (subset s1 s2)) = ()
+          
+let subset_mem (#a:eqtype) (s1 s2:set a)
+  : Lemma (requires (subset s1 s2))
+          (ensures (forall x. mem x s1 ==> mem x s2)) = ()
+          
 let rec remove_if (#a:eqtype) (s:set a) (f:a -> bool) =
   match s with
   |[] -> []
@@ -61,15 +80,6 @@ let rec remove_if_mem (#a:eqtype) (s:set a) (f:a -> bool) (x:a)
   |[] -> ()
   |x1::xs -> remove_if_mem xs f x
 
-let diff (#a:eqtype) (s1 s2:set a) : set a =
-  remove_if s1 (fun e -> mem e s2)
-
-let rec diff_mem (#a:eqtype) (s1 s2:set a) (x:a)
-  : Lemma (ensures mem x (diff s1 s2) <==> (mem x s1 /\ ~ (mem x s2)))  =
-  match s1 with
-  |[] -> ()
-  |x1::xs -> diff_mem xs s2 x
-  
 let rec filter_s (#a:eqtype) (s:set a) (f:a -> bool) =
   match s with
   |[] -> []
@@ -103,7 +113,7 @@ let rec forall_mem (#a:eqtype) (s:set a) (f:a -> bool)
   |[] -> ()
   |x::xs -> forall_mem xs f
 
-let extract (#a:Type0) (x:option a{Some? x}) : (r:a{x == Some r}) =
+(*let extract (#a:Type0) (x:option a{Some? x}) : (r:a{x == Some r}) =
   let (Some a) = x in a
 
 let rec find_if (#a:eqtype) (s:set a) (f:a -> bool) : option a =
@@ -214,4 +224,4 @@ let mem_remove_min_nat (s:set nat)
                    (s <> empty /\ Some? (find_min_nat s) ==> (forall e. mem e r <==> (mem e s /\ e <> extract (find_min_nat s)))) /\
                    (s <> empty /\ None? (find_min_nat s) ==> (forall e. mem e r <==> mem e s)))) = 
   always_min_exists_nat s
-  
+  *)
