interface/Set_extended.fsti
@@ -5,12 +5,12 @@ val t (a:eqtype) : Type0
 val empty (#a:eqtype) : t a
 val singleton (#a:eqtype) (x:a) : t a
 val mem (#a:eqtype) (x:a) (s:t a) : bool
-val equal (#a:eqtype) (s1 s2:t a) : Type0
+val equal (#a:eqtype) (s1:t a) (s2:t a) : Type0
 val union (#a:eqtype) (s1 s2:t a) : t a
 val intersection (#a:eqtype) (s1 s2:t a) : t a
 val difference (#a:eqtype) (s1 s2:t a) : t a
 val filter (#a:eqtype) (s:t a) (p:a -> bool) : t a
-val remove (#a:eqtype) (s:t a) (x:a) : t a
+//val remove (#a:eqtype) (s:t a) (x:a) : t a
 
 val mem_empty (#a:eqtype) (x:a)
   : Lemma (not (mem x empty))
@@ -72,12 +72,12 @@ val mem_filter (#a:eqtype) (s:t a) (p:a -> bool) (x:a)
   : Lemma (mem x (filter s p) <==> (mem x s /\ p x))
           [SMTPat (mem x (filter s p))]
 
-val mem_remove_x (#a:eqtype) (s:t a) (x:a)
+(*val mem_remove_x (#a:eqtype) (s:t a) (x:a)
   : Lemma (not (mem x (remove s x)))
           [SMTPat (mem x (remove s x))]
 
 val mem_remove_y (#a:eqtype) (s:t a) (x:a) (y:a)
   : Lemma (requires x =!= y)
           (ensures mem y (remove s x) == mem y s)
-          [SMTPat (mem y (remove s x))]
+          [SMTPat (mem y (remove s x))]*)
           
